apply_inner_complete

src/functional.lean
@@ -1,10 +1,11 @@
 -- functional.lean
 -- variability-aware functional programming
 --import .variability
-import data.fintype
+--import data.fintype
 import data.finset
 import tactic.basic
-import order.lattice
+import order.boolean_algebra
+import order.bounded_lattice
 
 namespace functional
 
@@ -20,11 +21,20 @@ inductive PC {Feature : Type} : Type
 | And  : PC → PC → PC
 | Or   : PC → PC → PC 
  
-def Config (Feature : Type) [fintype Feature] : finset Feature := 
-    fintype.elems Feature
+@[simp]
+def Config {Feature : Type} [fintype Feature] : finset Feature := 
+    finset.univ 
 
-def allConfigs (Feature : Type) [fintype Feature] 
-    := (Config Feature).powerset
+--instance fin_fin_power {α : Type} [t : fintype α]: fintype (finset (finset α)) :=
+--{ elems := finset.powerset (finset.univ.powerset) ,
+--  complete :=
+--  begin 
+--    intros, apply finset.subset_univ, apply finset.mem_univ
+--  end}
+
+@[simp]
+def allConfigs {Feature : Type} [t1 : fintype Feature] : finset (finset Feature)
+    := finset.univ 
 
 --def allProducts := allConfigs Feature L
 
@@ -33,14 +43,14 @@ open PC
 --@[simp]
 def semantics {Feature : Type} [fintype Feature] [decidable_eq Feature]
     : PC → finset (finset Feature)
-| (All) := allConfigs Feature
+| (All) := allConfigs
 | (None):= ∅
-| (Atom f)      := (allConfigs Feature).filter (λ p, f ∈ p)
-| (Not pc)      := (allConfigs Feature).filter (λ p, p ∈ (semantics pc))
+| (Atom f)      := allConfigs.filter (λ p, f ∈ p)
+| (Not pc)      := allConfigs.filter (λ p, p ∈ (semantics pc))
 | (And pc₁ pc₂) := (semantics pc₁) ∩ (semantics pc₂)
 | (Or  pc₁ pc₂) := (semantics pc₁) ∪ (semantics pc₂)
 
-structure Var {Feature: Type} [fintype Feature] (α : Type) := 
+structure Var {Feature: Type} [fintype Feature] {α : Type} := 
     (v : α) (pc : @PC Feature)
 
 --@[simp]
@@ -53,47 +63,48 @@ lemma conj_preserves_disjoint {Feature : Type} [fintype Feature] [decidable_eq F
     begin 
         --simp,   -- ∀ (pc₁ pc₂ c : PC), semantics (And pc₁ pc₂) = ∅ → 
                 -- semantics (And (And c pc₁) (And c pc₂)) = ∅ 
-        intros, -- semantics (And (And c pc₁) (And c pc₂)) = ∅
-        unfold disjoint, unfold disjoint at a,
+        intros pc₁ pc₂ c h, -- semantics (And (And c pc₁) (And c pc₂)) = ∅
+        unfold disjoint, unfold disjoint at h,
         unfold semantics, -- semantics c ∩ semantics pc₁ ∩ (semantics c ∩ semantics pc₂) = ∅
-        unfold semantics at a, -- a : semantics pc₁ ∩ semantics pc₂ = ∅ 
+        unfold semantics at h, -- a : semantics pc₁ ∩ semantics pc₂ = ∅ 
         simp, 
-        rw← finset.inter_assoc,
-        rw a, -- ∅ ∩ semantics c = ∅ 
-        apply finset.empty_inter
+        rw finset.inter_comm _ (semantics pc₂),
+        rw← finset.inter_assoc (semantics pc₁),
+        rw h, 
+        rw finset.empty_inter, simp 
     end
 
 --@[simp]
 def disjointList {Feature : Type} [t : fintype Feature] [decidable_eq Feature] {α : Type}
     (vs : list (@Var Feature t α)) : Prop :=
-    ∀ (x y : Var α) , x ∈ vs → y ∈ vs → x.pc ≠ y.pc → disjoint x.pc y.pc
+    ∀ (x y : Var) , x ∈ vs → y ∈ vs → x.pc ≠ y.pc → disjoint x.pc y.pc
 
 def cover {Feature : Type} [t : fintype Feature] [d : decidable_eq Feature] {α : Type}
     (v : list (@Var Feature t α)) := 
     semantics(list.foldr Or None (list.map (Var.pc) v))
 
-structure Lifted {Feature: Type} [fintype Feature] [decidable_eq Feature] (α : Type) := 
-    (s : list (Var α))
+structure Lifted {Feature: Type} [t : fintype Feature] [decidable_eq Feature] (α : Type) := 
+    (s : list (@Var Feature t α))
     (disj : disjointList s)
-    (comp : cover s = allConfigs Feature)
+    (comp : cover s = allConfigs)
 
 notation `⟦` p `⟧` := (semantics p)
 postfix `↑`:(max+1) := Lifted
 
 --@[simp]
-def apply_single {Feature : Type} [t: fintype Feature] [d: decidable_eq Feature] 
+def apply_single {Feature : Type} [t: fintype Feature] [d: decidable_eq Feature] {α β : Type}
     (f : @Var Feature t (α → β)) (u : α↑) : list (@Var Feature t β) :=
-    let sat := list.filter (λ(v : Var α), ⟦And f.pc v.pc⟧ ≠ ∅) u.s in
-    list.map (λ(v':Var α), Var.mk (f.v v'.v) (And f.pc  v'.pc)) sat
+    let sat := list.filter (λ(v : Var), ⟦And f.pc v.pc⟧ ≠ ∅) u.s in
+    list.map (λ(v':Var), Var.mk (f.v v'.v) (And f.pc  v'.pc)) sat
  
 lemma apply_single_disj {Feature : Type} [t: fintype Feature] [d: decidable_eq Feature] {α β : Type} : 
     ∀ (f : @Var Feature t (α → β)) (u : @Lifted Feature t d α), disjointList (apply_single f u) :=
 begin
     unfold apply_single, simp,
-    intros, unfold disjointList, simp, intros, 
-    rw[←a_2,←a_5], simp, apply conj_preserves_disjoint,
-    apply u.disj, apply a, apply a_3,
-    rw [←a_2, ←a_5] at a_6, simp at a_6, apply a_6
+    intros f u, unfold disjointList, simp, intros x y x₁ h₁ h₂ h₃ x₂ h₄ h₅ h₆ h₇, 
+    rw[←h₃,←h₆], simp, apply conj_preserves_disjoint,
+    apply u.disj, exact h₁, exact h₄,
+    rw [←h₃, ←h₆] at h₇, simp at h₇, apply h₇
 end
 
 section 
@@ -119,8 +130,8 @@ begin
     },
     {
         rw (if_pos hNEmpty), simp at ih, simp, unfold cover, simp, unfold cover at ih, 
-        unfold semantics, unfold semantics at ih, simp at ih, simp, rw ih,
-        rw finset.inter_distrib_left, simp     
+        unfold semantics, unfold semantics at ih, simp at ih, rw ih,
+        rw finset.inter_distrib_left     
     }
     
 end -- section
@@ -169,15 +180,17 @@ begin
     unfold cover, simp, unfold semantics, unfold cover at l₁_ih, simp at l₁_ih, 
     rw l₁_ih, rw← finset.union_assoc, cc 
 end
- 
+--#print finset.has_lift.lift
+#check finset.inter_univ
+
 lemma interAll {α : Type} {c: finset α} [d: decidable_eq α] [t: fintype α]:
-    (c.to_set) ∩ (finset.to_set (finset.univ)) = (c.to_set) := 
+    (c ∩ finset.univ) = c := 
 begin
     intros, --lift finset.univ to (set α) using finset.lift,
-    apply set.inter_eq_self_of_subset_left, unfold finset.to_set, simp, 
-    apply set.subset_univ 
+    --finish[set.inter_eq_self_of_subset_left],
+    apply finset.inter_univ
 end 
-
+ 
 lemma apply_inner_complete {Feature : Type} [t: fintype Feature] [d: decidable_eq Feature] {α β : Type} : 
     ∀ (f : @Lifted Feature t d (α → β)) (v : @Lifted Feature t d α),
     cover (apply_inner f v) = cover f.s :=
@@ -186,13 +199,8 @@ begin
     -- base case
     simp, refl,
     -- induction,
-    simp, rw cover_append, simp at ih, rw ih, rw apply_single_cover, rw v.comp, --rw← finset.inf_eq_inter,
-    --unfold allConfigs, unfold Config, rw← finset.univ, unfold finset.powerset, rw set.inter_univ,
-    rw interAll, 
-    unfold finset.inter, 
-    --set.inter_eq_self_of_subset_left,
-    simp, unfold finset.has_inter.inter, 
-    unfold cover, simp, unfold semantics, apply v.comp,    
+    simp, rw cover_append, simp at ih, rw ih, rw apply_single_cover, rw v.comp,
+    simp, unfold cover, simp, unfold semantics   
 end
 
 def apply {Feature : Type} [t: fintype Feature] [d: decidable_eq Feature] 
